Hs/Translator/Lemmas/TypesSoundness.lean
@@ -7,16 +7,19 @@ import Hs.Translator.HsTerm
 import Hs.SynthInstance
 
 import SystemFD.Term
+import SystemFD.Metatheory.Shape
+
 import Batteries.Lean.Except
 
 
 theorem synth_coercion_type_sound : ⊢ Γ ->
-  Term.IsType A ->
-  Term.IsType B ->
+  Term.isType Γ A ->
+  Term.isType Γ B ->
   infer_kind Γ A = .some k ->
   infer_kind Γ B = .some k ->
-  synth_coercion Γ A B = .some t -> Γ ⊢ t : (A ~[k]~ B) := by
-intro wf wfA wfB jAk jBk j
+  synth_coercion Γ A B = .some t ->
+  Γ ⊢ t : (A ~[k]~ B) := by
+intro wf wflhs wfrhs jlhsk jrhsk j
 induction Γ, A, B using synth_coercion.induct generalizing t k
 all_goals (
   unfold synth_coercion at j; simp at j; rw[Option.bind_eq_some] at j
@@ -35,28 +38,28 @@ case _ ih1 ih2 _ j => -- A1 `@k B1 ~ A2 `@k B2
   case _ kA1 jA1 kA2 jA2 kB1 jB1 kB2 jB2 jes w1 j1 w2 j2 =>
   have j3 := Term.eq_of_beq jes.1
   have j4 := Term.eq_of_beq jes.2
-  unfold infer_kind at jAk; simp at jAk;
-  rw[Option.bind_eq_some] at jAk; cases jAk; case _ jAk =>
-  rw[Option.bind_eq_some] at jAk; cases jAk; case _ jAk =>
-  cases jAk; case _ jAk =>
-  rw[Option.bind_eq_some] at jAk; cases jAk; case _ jAk =>
-  cases jAk; case _ jAk =>
-  cases jAk; case _ jAk =>
-  simp at jAk;
-  cases jAk
+  unfold infer_kind at jlhsk; simp at jlhsk;
+  rw[Option.bind_eq_some] at jlhsk; cases jlhsk; case _ jlhsk =>
+  rw[Option.bind_eq_some] at jlhsk; cases jlhsk; case _ jlhsk =>
+  cases jlhsk; case _ jlhsk =>
+  rw[Option.bind_eq_some] at jlhsk; cases jlhsk; case _ jlhsk =>
+  cases jlhsk; case _ jlhsk =>
+  cases jlhsk; case _ jlhsk =>
+  simp at jlhsk;
+  cases jlhsk
   case _ A1k kk arrK _ B1k eA1 eA2 =>
   have lem := is_arrowk_some arrK;
   cases lem; unfold is_arrowk at arrK; simp at arrK;
   have lemA1 := infer_kind_sound A1k wf;
   cases eA2
-  unfold infer_kind at jBk; simp at jBk;
-  rw[Option.bind_eq_some] at jBk; cases jBk; case _ jBk =>
-  rw[Option.bind_eq_some] at jBk; cases jBk; case _ jBk =>
-  cases jBk; case _ jBk =>
-  rw[Option.bind_eq_some] at jBk; cases jBk; case _ jBk =>
-  cases jBk; case _ jBk =>
-  cases jBk; case _ jBk =>
-  simp at jBk; cases jBk;
+  unfold infer_kind at jrhsk; simp at jrhsk;
+  rw[Option.bind_eq_some] at jrhsk; cases jrhsk; case _ jrhsk =>
+  rw[Option.bind_eq_some] at jrhsk; cases jrhsk; case _ jrhsk =>
+  cases jrhsk; case _ jrhsk =>
+  rw[Option.bind_eq_some] at jrhsk; cases jrhsk; case _ jrhsk =>
+  cases jrhsk; case _ jrhsk =>
+  cases jrhsk; case _ jrhsk =>
+  simp at jrhsk; cases jrhsk;
   case _ A2k kk2 arr2K _ B2k eB1 eB2 =>
   have lem := is_arrowk_some arr2K;
   cases lem; unfold is_arrowk at arr2K; simp at arr2K;
@@ -65,35 +68,97 @@ case _ ih1 ih2 _ j => -- A1 `@k B1 ~ A2 `@k B2
   replace eB1 := Term.eq_of_beq eB1;
   replace eA1 := Term.eq_of_beq eA1;
   cases eB1; cases eA1;
-  cases wfA; cases wfB;
-  case _ h1 h2 _ _ h3 h4 =>
-  have ih1' := @ih1 (kk.fst -k> kk.snd) w1 wf h1 h3
-
+  unfold Term.isType at wflhs; simp at wflhs;
+  unfold Term.isType at wfrhs; simp at wfrhs;
+  cases wflhs; cases wfrhs;
   simp_all;
-  apply Judgment.appc; sorry; sorry; sorry
+  apply Judgment.appc; assumption; assumption
 
-· sorry -- A1 -t> B1 ~ A2 -t> B2
-· sorry
+case _ ih1 ih2 _ j => -- A1 -t> B1 ~ A2 -t> B2
+  cases j; case _ j =>
+  rw[Option.bind_eq_some] at j; cases j; case _ j =>
+  rw[Option.bind_eq_some] at j; cases j; case _ j =>  cases j; case _ j =>
+  rw[Option.bind_eq_some] at j; cases j; case _ j =>  cases j; case _ j =>
+  cases j; case _ j =>
+  simp at j; cases j; case _ j =>
+  rw[Option.bind_eq_some] at j; cases j; case _ j =>  cases j; case _ j =>
+  rw[Option.bind_eq_some] at j; cases j; case _ j =>  cases j; case _ j =>
+  cases j
+  case _ kA1 jA1 kA2 jA2 kB1 jB1 kB2 jB2 jes w1 j1 w2 j2 =>
+  have j3 := Term.eq_of_beq jes.1
+  have j4 := Term.eq_of_beq jes.2
+  cases j3; cases j4; clear jes
+  have jAk' := infer_kind_sound jlhsk wf
+  have jrhsk' := infer_kind_sound jrhsk wf
+  cases jAk'; cases jrhsk'
+  unfold Term.isType at wflhs; simp at wflhs
+  unfold Term.isType at wfrhs; simp at wfrhs
+  case _ jA1k jB1k jA2k jB2k =>
+  have lemA1k := infer_kind_sound jA1 wf
+  have lemB1k := infer_kind_sound jB1 (Judgment.wfempty wf)
+  have lemA2k := infer_kind_sound jA2 wf
+  have lemB2k := infer_kind_sound jB2 (Judgment.wfempty wf)
+  have u := uniqueness_of_kinds (Term.is_type_shape_sound wflhs.1) lemA1k jA1k; cases u
+  have u := uniqueness_of_kinds (Term.is_type_shape_sound wflhs.1) lemA1k jA1k; cases u
+  have u := uniqueness_of_kinds (Term.is_type_shape_sound wflhs.2) lemB1k jB1k; cases u
+  have u := uniqueness_of_kinds (Term.is_type_shape_sound wfrhs.2) lemB2k jB2k; cases u
+  have ih1' := @ih1 ★ w1 wf wflhs.1 wfrhs.1 jA1 jA2 j1
+  have ih2' := @ih2 ★ w2 (Judgment.wfempty wf) wflhs.2 wfrhs.2 jB1 jB2 j2
+  constructor; assumption;  assumption
+
+case _ K1 _ _ _ ih _ j => -- Γ ⊢ t : ((∀[K1]A1) ~[k]~ ∀[K2]A2)
+  cases j; case _ j =>
+  rw[Option.bind_eq_some] at j; cases j; case _ j =>
+  cases j; case _ j =>
+  rw[Option.bind_eq_some] at j; cases j; case _ j =>
+  cases j; case _ j =>
+  rw[Option.bind_eq_some] at j; cases j; case _ j =>
+  cases j; case _ j =>
+  simp at j; cases j; case _ j =>
+  rw[Option.bind_eq_some] at j; cases j; case _ j =>
+  cases j; case _ j =>
+  cases j; case _  j1 _ j2 _ j3 _ j4 j5 w j6 =>
+  replace j5 := Term.eq_of_beq j5; cases j5
+  have j1' := wf_kind_sound j1 wf
+  clear j2;
+  have lem' := infer_kind_sound jrhsk wf
+  cases lem'; case _ lemlhs =>
+  have lem' := infer_kind_sound jlhsk wf
+  cases lem'; case _ lemrhs =>
+  have wf' := Judgment.wfkind j1' wf
+  unfold Term.isType at wflhs; simp at wflhs
+  unfold Term.isType at wfrhs; simp at wfrhs
+  have lemA1 := infer_kind_sound j3 (Judgment.wfkind j1' wf)
+  have lemA2 := infer_kind_sound j4 (Judgment.wfkind j1' wf)
+  have u := uniqueness_of_kinds (Term.is_type_shape_sound wflhs.2) lemrhs lemA1; cases u
+  have u := uniqueness_of_kinds (Term.is_type_shape_sound wfrhs.2) lemlhs lemA2; cases u
+  case _  jB1k _ jB2k =>
+  have ih1' := @ih ★ w (Judgment.wfkind j1' wf) wflhs.2 wfrhs.2 j3 j4 j6
+  constructor; assumption; assumption
+
 case _ j =>
  cases j; case _ j =>
  simp at j; split at j
  · cases j; case _ j =>
    replace j := Term.eq_of_beq j; cases j
    case _ k jlhs _ _ _ =>
-   rw[jlhs] at jBk; cases jBk
+   rw[jlhs] at jrhsk; cases jrhsk
    constructor
-   · have lem := infer_kind_sound jAk wf;
-
-     sorry
+   · have lem1 := infer_kind_sound jlhsk wf;
+     have lem2 := Term.is_type_shape_sound wfrhs
+     have lem3 := kind_of_type_well_formed wf lem2 lem1
+     assumption
    · apply infer_kind_sound jlhs wf
  · rw[Option.bind_eq_some] at j; cases j; case _ j =>
    cases j; case _ j1 j2 => sorry -- needs coercion_graph_kind_soundness etc.
 
 
 theorem synth_term_type_sound : ⊢ Γ ->
+  Term.isType Γ τ ->
+  Term.isKind k ->
   Γ ⊢ τ : k ->
   synth_term n Γ τ = .some t -> Γ ⊢ t : τ := by
-intro wf jk j
+intro wf wfτ wfk jk j
 induction n, τ using synth_term.induct generalizing Γ t
 all_goals (unfold synth_term at j)
 · simp at j;
@@ -107,11 +172,60 @@ all_goals (unfold synth_term at j)
   case _ e _ =>
   replace e := Term.eq_of_beq e; cases e;
   case _ =>
-  apply synth_coercion_type_sound; assumption; sorry; sorry; sorry
-· sorry
-· sorry
+    unfold Term.isType at wfτ; simp at wfτ;
+    cases wfτ; case _ wfτ _ =>
+    cases wfτ; cases jk;
+    case _ j1 _ j2 j3 j4 j5 j6 j7 j8 =>
+    have lemA := infer_kind_sound j1 wf
+    have lemB := infer_kind_sound j2 wf
+    have lemA' := Term.is_type_shape_sound j4
+    have lemB' := Term.is_type_shape_sound j5
+    have u := uniqueness_of_kinds lemA' j7 lemA; cases u
+    have u := uniqueness_of_kinds lemB' j8 lemB; cases u
+    apply synth_coercion_type_sound; assumption; assumption; assumption; assumption; assumption; assumption
+· simp at j;
+  cases j;
+  case _ ih1 ih2 _ j =>
+  rw[Option.bind_eq_some] at j; cases j; case _ j =>
+  cases j; case _ j =>
+  rw[Option.bind_eq_some] at j; cases j; case _ j =>
+  cases j; case _ j =>
+  simp at j; cases j;
+  case _ e _ =>
+  replace e := Term.eq_of_beq e; cases e;
+  case _ j _ =>
+  split at j
+  case _ => cases j; sorry
+  case _ =>
+    sorry
+    -- unfold Term.isType at wfτ; simp at wfτ;
+    -- cases wfτ; case _ wfτ _ =>
+    -- cases wfτ; cases jk;
+    -- case _ j1 _ j2 j3 j4 j5 j6 j7 j8 =>
+    -- have lemA := infer_kind_sound j1 wf
+    -- have lemB := infer_kind_sound j2 wf
+    -- have lemA' := Term.is_type_shape_sound j4
+    -- have lemB' := Term.is_type_shape_sound j5
+    -- have u := uniqueness_of_kinds lemA' j7 lemA; cases u
+    -- have u := uniqueness_of_kinds lemB' j8 lemB; cases u
+    -- apply synth_coercion_type_sound; assumption; assumption; assumption; assumption; assumption; assumption
+    -- · simp at j;
+    --   cases j;
+    -- sorry
+
 case _ h =>
   unfold synth_term at j; simp at j; exfalso; simp_all;
+  cases j; case _ j =>
+  simp at j;
+  rw[Option.bind_eq_some] at j; cases j; case _ j =>
+  cases j; case _ j =>
+  rw[Option.bind_eq_some] at j; cases j; case _ j =>
+  cases j; case _ j =>
+  rw[Option.bind_eq_some] at j; cases j; case _ j =>
+  cases j; case _ j1 j2 =>
+  sorry
+case _ => simp_all -- contradiction case we are out of corns
+
 
 
 theorem compile_type_sound (k : Term) (τ : HsTerm) :
@@ -187,7 +301,7 @@ case _ k τ sp h tnfp tnf _ _ _ ih =>
       have lem := dsm_get_type_sound wf t1;
       -- we are stuck here. as we do not know the shape of w1
       sorry
-    · sorry
+    · cases j
 
   case _ tnf ih =>
   rw[tnf] at e; cases e;
